L6 event conversion. Update ErrSID to not depend on LLVM_INTERACTIONS. Move some things (like ltac for solving measures (dtyp_measure, dvalue_measure, uvalue_measure) around.

src/coq/Semantics/InfiniteToFinite.v
@@ -19,7 +19,10 @@ From Vellvm Require Import
 From ExtLib Require Import
      Structures.Monads.
 
-From ITree Require Import Basics.Basics ITrace.EuttEv.
+From ITree Require Import
+     ITree
+     Basics.Basics
+     ITrace.EuttEv.
 
 Import MonadNotation.
 
@@ -27,13 +30,19 @@ Module Type AddrConvert (LP1 : LLVMParams) (LP2 : LLVMParams).
   Parameter addr_convert : LP1.ADDR.addr -> OOM LP2.ADDR.addr.
 End AddrConvert.
 
-Module DVConvert (LP1 : LLVMParams) (LP2 : LLVMParams) (AC : AddrConvert LP1 LP2) (Events1 : LLVM_INTERACTIONS LP1.ADDR LP1.IP LP1.SIZEOF) (Events2 : LLVM_INTERACTIONS LP2.ADDR LP2.IP LP2.SIZEOF).
+Module Type DVConvert (LP1 : LLVMParams) (LP2 : LLVMParams) (AC : AddrConvert LP1 LP2) (Events1 : LLVM_INTERACTIONS LP1.ADDR LP1.IP LP1.SIZEOF) (Events2 : LLVM_INTERACTIONS LP2.ADDR LP2.IP LP2.SIZEOF).
+  Parameter dvalue_convert : Events1.DV.dvalue -> OOM Events2.DV.dvalue.
+  Parameter uvalue_convert : Events1.DV.uvalue -> OOM Events2.DV.uvalue.
+End DVConvert.
+
+Module DVConvertMake (LP1 : LLVMParams) (LP2 : LLVMParams) (AC : AddrConvert LP1 LP2) (Events1 : LLVM_INTERACTIONS LP1.ADDR LP1.IP LP1.SIZEOF) (Events2 : LLVM_INTERACTIONS LP2.ADDR LP2.IP LP2.SIZEOF) : DVConvert LP1 LP2 AC Events1 Events2.
   Import AC.
 
   Module DV1 := Events1.DV.
   Module DV2 := Events2.DV.
 
-  Obligation Tactic := try Tactics.program_simpl; try solve [cbn; try lia | DV1.solve_dvalue_measure].
+  Obligation Tactic := try Tactics.program_simpl; try solve [cbn; try lia | DV1.solve_dvalue_measure | DV1.solve_uvalue_measure].
+
   Program Fixpoint dvalue_convert (dv1 : DV1.dvalue) {measure (DV1.dvalue_measure dv1)} : OOM DV2.dvalue
     := match dv1 with
        | DV1.DVALUE_Addr a =>
@@ -64,7 +73,147 @@ Module DVConvert (LP1 : LLVMParams) (LP2 : LLVMParams) (AC : AddrConvert LP1 LP2
            elts' <- map_monad_In elts (fun elt Hin => dvalue_convert elt);;
            ret (DV2.DVALUE_Vector elts')
        end.
-End DVConvert.
+
+  Program Fixpoint uvalue_convert (uv1 : DV1.uvalue) {measure (DV1.uvalue_measure uv1)} : OOM DV2.uvalue
+    := match uv1 with
+       | DV1.UVALUE_Addr a =>
+           a' <- addr_convert a;;
+           ret (DV2.UVALUE_Addr a')
+       | DV1.UVALUE_I1 x  => ret (DV2.UVALUE_I1 x)
+       | DV1.UVALUE_I8 x  => ret (DV2.UVALUE_I8 x)
+       | DV1.UVALUE_I32 x => ret (DV2.UVALUE_I32 x)
+       | DV1.UVALUE_I64 x => ret (DV2.UVALUE_I64 x)
+       | DV1.UVALUE_IPTR x =>
+           let xz := LP1.IP.to_Z x in
+           x' <- LP2.IP.from_Z xz;;
+           ret (DV2.UVALUE_IPTR x')
+       | DV1.UVALUE_Double x => ret (DV2.UVALUE_Double x)
+       | DV1.UVALUE_Float x => ret (DV2.UVALUE_Float x)
+       | DV1.UVALUE_Poison t => ret (DV2.UVALUE_Poison t)
+       | DV1.UVALUE_None => ret DV2.UVALUE_None
+       | DV1.UVALUE_Struct fields =>
+           fields' <- map_monad_In fields (fun elt Hin => uvalue_convert elt);;
+           ret (DV2.UVALUE_Struct fields')
+       | DV1.UVALUE_Packed_struct fields =>
+           fields' <- map_monad_In fields (fun elt Hin => uvalue_convert elt);;
+           ret (DV2.UVALUE_Packed_struct fields')
+       | DV1.UVALUE_Array elts =>
+           elts' <- map_monad_In elts (fun elt Hin => uvalue_convert elt);;
+           ret (DV2.UVALUE_Array elts')
+       | DV1.UVALUE_Vector elts =>
+           elts' <- map_monad_In elts (fun elt Hin => uvalue_convert elt);;
+           ret (DV2.UVALUE_Vector elts')
+       | DV1.UVALUE_Undef dt =>
+           (* Could be a bit odd with intptr *)
+           ret (DV2.UVALUE_Undef dt)
+       | DV1.UVALUE_IBinop iop v1 v2 =>
+           v1' <- uvalue_convert v1;;
+           v2' <- uvalue_convert v2;;
+           ret (DV2.UVALUE_IBinop iop v1' v2')
+       | DV1.UVALUE_ICmp cmp v1 v2 =>
+           v1' <- uvalue_convert v1;;
+           v2' <- uvalue_convert v2;;
+           ret (DV2.UVALUE_ICmp cmp v1' v2')
+       | DV1.UVALUE_FBinop fop fm v1 v2 =>
+           v1' <- uvalue_convert v1;;
+           v2' <- uvalue_convert v2;;
+           ret (DV2.UVALUE_FBinop fop fm v1' v2')
+       | DV1.UVALUE_FCmp cmp v1 v2 =>
+           v1' <- uvalue_convert v1;;
+           v2' <- uvalue_convert v2;;
+           ret (DV2.UVALUE_FCmp cmp v1' v2')
+       | DV1.UVALUE_Conversion conv t_from v t_to =>
+           v' <- uvalue_convert v;;
+           ret (DV2.UVALUE_Conversion conv t_from v' t_to)
+       | DV1.UVALUE_GetElementPtr t ptrval idxs =>
+           ptrval' <- uvalue_convert ptrval;;
+           idxs' <- map_monad_In idxs (fun elt Hin => uvalue_convert elt);;
+           ret (DV2.UVALUE_GetElementPtr t ptrval' idxs')
+       | DV1.UVALUE_ExtractElement vec idx =>
+           vec' <- uvalue_convert vec;;
+           idx' <- uvalue_convert idx;;
+           ret (DV2.UVALUE_ExtractElement vec' idx')
+       | DV1.UVALUE_InsertElement vec elt idx =>
+           vec' <- uvalue_convert vec;;
+           elt' <- uvalue_convert elt;;
+           idx' <- uvalue_convert idx;;
+           ret (DV2.UVALUE_InsertElement vec' elt' idx')
+       | DV1.UVALUE_ShuffleVector vec1 vec2 idxmask =>
+           vec1' <- uvalue_convert vec1;;
+           vec2' <- uvalue_convert vec2;;
+           idxmask' <- uvalue_convert idxmask;;
+           ret (DV2.UVALUE_ShuffleVector vec1' vec2' idxmask')
+       | DV1.UVALUE_ExtractValue vec idxs =>
+           vec' <- uvalue_convert vec;;
+           ret (DV2.UVALUE_ExtractValue vec' idxs)
+       | DV1.UVALUE_InsertValue vec elt idxs =>
+           vec' <- uvalue_convert vec;;
+           elt' <- uvalue_convert elt;;
+           ret (DV2.UVALUE_InsertValue vec' elt' idxs)
+       | DV1.UVALUE_Select cnd v1 v2 =>
+           cnd' <- uvalue_convert cnd;;
+           v1' <- uvalue_convert v1;;
+           v2' <- uvalue_convert v2;;
+           ret (DV2.UVALUE_Select cnd' v1' v2')
+       | DV1.UVALUE_ExtractByte uv dt idx sid =>
+           uv' <- uvalue_convert uv;;
+           idx' <- uvalue_convert idx;;
+           ret (DV2.UVALUE_ExtractByte uv' dt idx' sid)
+       | DV1.UVALUE_ConcatBytes uvs dt =>
+           uvs' <- map_monad_In uvs (fun elt Hin => uvalue_convert elt);;
+           ret (DV2.UVALUE_ConcatBytes uvs' dt)
+       end.
+
+End DVConvertMake.
+
+Module Type EventConvert (LP1 : LLVMParams) (LP2 : LLVMParams) (AC : AddrConvert LP1 LP2) (AC2 : AddrConvert LP2 LP1) (E1 : LLVM_INTERACTIONS LP1.ADDR LP1.IP LP1.SIZEOF) (E2 : LLVM_INTERACTIONS LP2.ADDR LP2.IP LP2.SIZEOF).
+  (* TODO: should this be a parameter? *)
+  Module DVC := DVConvertMake LP1 LP2 AC E1 E2.
+  Module DVCrev := DVConvertMake LP2 LP1 AC2 E2 E1.
+  Import DVC.
+
+  Definition OOM_to_OOME_NOMSG {E} `{OOME_NOMSG -< E} (m : OOM (E void)) : E void
+    := match m with
+       | NoOom e => e
+       | Oom msg => subevent _ ThrowOOM_NOMSG
+       end.
+
+  Require Import String.
+
+  Definition L6_convert : Handler E1.L6 E2.L6.
+  Proof.
+    refine (fun A e => _).
+
+    refine (match e with
+            | inl1 (E1.ExternalCall dt f args) =>
+                _
+            | inr1 (inl1 e0) =>
+                raise_oom ""
+            | inr1 (inr1 (inl1 e0)) =>
+                _
+            | inr1 (inr1 (inr1 e0)) =>
+                _
+            end).
+
+    (* External Calls *)
+    refine (f' <- lift_OOM (uvalue_convert f);;
+            args' <- lift_OOM (map_monad_In args (fun elt Hin => dvalue_convert elt));;
+            dv <- trigger (E2.ExternalCall dt f' args');;
+            _).
+
+    inversion e0.
+    apply (lift_OOM (DVCrev.dvalue_convert dv)).
+
+    (* DebugE *)
+    inversion e0.
+    apply (debug H).
+
+    (* FailureE *)
+    inversion e0.
+    unfold FailureE in e0.
+    apply (raise_error "").
+  Defined.  
+End EventConvert.
 
 Module InfiniteToFinite (IS1 : InterpreterStack) (IS2 : InterpreterStack) (LLVM1 : LLVMTopLevel IS1) (LLVM2 : LLVMTopLevel IS2).
 
